examples/CleanSTLC.v
@@ -17,7 +17,7 @@ Inductive value : term -> Prop :=
 
 Inductive bind_val : list (nat * term) -> nat -> term -> Prop :=
 | bv_here : forall env v t, bind_val ((v,t) :: env) v t 
-| bv_later : forall env v t v' t', v <> v' -> bind_val env v t -> bind_val ((v',t') :: env) v t 
+| bv_later : forall env v t v' t', v <> v' -> True -> bind_val env v t -> bind_val ((v',t') :: env) v t 
 .
 
 Require Import Init Arith Logic Bool List.
@@ -98,9 +98,13 @@ Inductive bind_typ : list (nat * typ) -> nat -> typ -> Prop :=
 .
 
 Inductive typing (g : list (nat * typ)) : term -> typ -> Prop :=
-| typ_var : forall x ty, bind_typ g x ty -> typing g (Var x) ty
-| typ_abs : forall x t body tbody, typing ((x,t) :: g) body tbody -> typing g (Abs x t body) (TArrow t tbody)
-| typ_app : forall fe xe tfrom tto, typing g fe (TArrow tfrom tto) -> typing g xe tfrom -> typing g (App fe xe) tto
+| typ_var : forall x ty, bind_typ g x ty ->
+                         typing g (Var x) ty
+| typ_abs : forall x t body tbody, typing ((x,t) :: g) body tbody ->
+                                   typing g (Abs x t body) (TArrow t tbody)
+| typ_app : forall fe xe tfrom tto, typing g fe (TArrow tfrom tto) ->
+                                    typing g xe tfrom ->
+                                    typing g (App fe xe) tto
 | typ_const : forall n, typing g (Const n) TNat
 .
 
@@ -114,7 +118,7 @@ Proof.
   theorem_dependencies.
   Derive Used Inds smallstep.
   Derive Used Inds typing.
-  Derive Density typing.
+  Derive Density typing derive "Gen".
   Abort. 
 
 
@@ -124,89 +128,638 @@ Theorem typ_abs' :  forall g x t body tbody, typing ((x,t) :: g) body tbody ->
   theorem_dependencies.
   QuickChickDebug Debug Off.
   schedules.
-  valid_schedules.
-  Derive Schedules typing 1  consnum 1.
-  Derive Valid Schedules typing 1 consnum 2.
-  Derive Inductive Schedule typing derive "Check" opt "true". Check @bind.
+  (*valid_schedules.*)
+  (*Derive Schedules typing 1  consnum 1.*) Locate eq.
+  Derive Valid Schedules eq consnum 0 derive "Check".
 
-Check (let EnumSizedSuchThattyping_IOOEnum :=
-   fix rec
-     (init_size : Coq.Init.Datatypes.nat) (size : Coq.Init.Datatypes.nat) (v_g5142_ : @list (@prod (@nat) (@typ))) 
-     (v5143_ : @term) (v5144_ : @typ) :=
+  Derive Inductive Schedule Coq.Init.Logic.eq  derive "Check" opt "true". 
+
+  Derive Show for typ. Derive EnumSized for typ.
+Print EnumSizedtyp. Locate oneOf_. Print QuickChick.Enumerators. Check @oneOf_.
+Compute ((let EnumSizedtyp_Enum :=
+   fix rec (init_size : Coq.Init.Datatypes.nat) (size : Coq.Init.Datatypes.nat) :=
      match size with
      | @Coq.Init.Datatypes.O =>
-         @QuickChick.Enumerators.enumerate _
-           (@Coq.Init.Datatypes.cons _
-              (@QuickChick.Producer.bindOpt _ _ _ _
-                 (@QuickChick.DependentClasses.enumSizeST _
-                    (fun '(@Coq.Init.Datatypes.pair _ _ v5144_ x) => @bind_typ v_g5142_ x v5144_) _ init_size)
-                 (fun '(@Coq.Init.Datatypes.pair _ _ v5144_ x) =>
-                  @QuickChick.Enumerators.returnEnum _ (@Coq.Init.Datatypes.Some _ (@Coq.Init.Datatypes.pair _ _ (@Var x) v5144_))))
-              (@Coq.Init.Datatypes.cons _
-                 (@QuickChick.Producer.bindOpt _ _ _ _
-                    (@QuickChick.DependentClasses.enumSizeST _
-                       (fun '(@Coq.Init.Datatypes.pair _ _ (@Coq.Init.Datatypes.pair _ _ (@Coq.Init.Datatypes.pair _ _ body t) tbody) x)
-                        =>
-                        @typing (@Coq.Init.Datatypes.cons (@prod (@nat) (@typ)) (@Coq.Init.Datatypes.pair (@nat) (@typ) x t) v_g5142_)
-                          body tbody) _ init_size)
-                    (fun '(@Coq.Init.Datatypes.pair _ _ (@Coq.Init.Datatypes.pair _ _ (@Coq.Init.Datatypes.pair _ _ body t) tbody) x) =>
-                     @QuickChick.Enumerators.returnEnum _
-                       (@Coq.Init.Datatypes.Some _ (@Coq.Init.Datatypes.pair _ _ (@Abs x t body) (@TArrow t tbody)))))
-                 (@Coq.Init.Datatypes.cons _
-                    (@QuickChick.Producer.bindOpt _ _ _ _
-                       (@QuickChick.DependentClasses.enumSizeST _
-                          (fun '(@Coq.Init.Datatypes.pair _ _ fe tfromto) => @typing v_g5142_ fe tfromto) _ init_size)
-                       (fun '(@Coq.Init.Datatypes.pair _ _ fe tfromto) =>
-                        @QuickChick.Producer.bindOpt _ _ _ _
-                          (@QuickChick.DependentClasses.enumSizeST _
-                             (fun '(@Coq.Init.Datatypes.pair _ _ tfrom xe) => @typing v_g5142_ xe tfrom) _ init_size)
-                          (fun '(@Coq.Init.Datatypes.pair _ _ tfrom xe) =>
-                           @QuickChick.Enumerators.bindEnum _ _ (@QuickChick.Classes.enumSized (@typ) _ init_size)
-                             (fun 'v5144_ =>
-                              @QuickChick.Enumerators.returnEnum _
-                                (@Coq.Init.Datatypes.Some _ (@Coq.Init.Datatypes.pair _ _ (@App fe xe) v5144_))))))
-                    (@Coq.Init.Datatypes.cons _
-                       (@QuickChick.Enumerators.bindEnum _ _ (@QuickChick.Classes.enumSized (@nat) _ init_size)
-                          (fun 'n =>
-                           @QuickChick.Enumerators.returnEnum _
-                             (@Coq.Init.Datatypes.Some _ (@Coq.Init.Datatypes.pair _ _ (@Const n) (@TNat)))))
-                       (@Coq.Init.Datatypes.nil _)))))
+         @QuickChick.Producer.oneOf_ _ _ _ (@QuickChick.Enumerators.returnEnum _ (@TNat))
+           (@Coq.Init.Datatypes.cons _ (@QuickChick.Enumerators.returnEnum _ (@TNat)) (@Coq.Init.Datatypes.nil _))
      | @Coq.Init.Datatypes.S size' =>
-         @QuickChick.Enumerators.enumerate _
-           (@Coq.Init.Datatypes.cons _
-              (@QuickChick.Producer.bindOpt _ _ _ _
-                 (@QuickChick.DependentClasses.enumSizeST _
-                    (fun '(@Coq.Init.Datatypes.pair _ _ v5144_ x) => @bind_typ v_g5142_ x v5144_) _ init_size)
-                 (fun '(@Coq.Init.Datatypes.pair _ _ v5144_ x) =>
-                  @QuickChick.Enumerators.returnEnum _ (@Coq.Init.Datatypes.Some _ (@Coq.Init.Datatypes.pair _ _ (@Var x) v5144_))))
+         @QuickChick.Producer.oneOf_ _ _ _ (@QuickChick.Enumerators.returnEnum _ (@TNat))
+           (@Coq.Init.Datatypes.cons _ (@QuickChick.Enumerators.returnEnum _ (@TNat))
               (@Coq.Init.Datatypes.cons _
-                 (@QuickChick.Producer.bindOpt _ _ _ _
-                    (@QuickChick.DependentClasses.enumSizeST _
-                       (fun '(@Coq.Init.Datatypes.pair _ _ (@Coq.Init.Datatypes.pair _ _ (@Coq.Init.Datatypes.pair _ _ body t) tbody) x)
-                        =>
-                        @typing (@Coq.Init.Datatypes.cons (@prod (@nat) (@typ)) (@Coq.Init.Datatypes.pair (@nat) (@typ) x t) v_g5142_)
-                          body tbody) _ init_size)
-                    (fun '(@Coq.Init.Datatypes.pair _ _ (@Coq.Init.Datatypes.pair _ _ (@Coq.Init.Datatypes.pair _ _ body t) tbody) x) =>
-                     @QuickChick.Enumerators.returnEnum _
-                       (@Coq.Init.Datatypes.Some _ (@Coq.Init.Datatypes.pair _ _ (@Abs x t body) (@TArrow t tbody)))))
-                 (@Coq.Init.Datatypes.cons _
-                    (@QuickChick.Producer.bindOpt _ _ _ _
-                       (@QuickChick.DependentClasses.enumSizeST _
-                          (fun '(@Coq.Init.Datatypes.pair _ _ fe tfromto) => @typing v_g5142_ fe tfromto) _ init_size)
-                       (fun '(@Coq.Init.Datatypes.pair _ _ fe tfromto) =>
-                        @QuickChick.Producer.bindOpt _ _ _ _
-                          (@QuickChick.DependentClasses.enumSizeST _
-                             (fun '(@Coq.Init.Datatypes.pair _ _ tfrom xe) => @typing v_g5142_ xe tfrom) _ init_size)
-                          (fun '(@Coq.Init.Datatypes.pair _ _ tfrom xe) =>
-                           @QuickChick.Enumerators.bindEnum _ _ (@QuickChick.Classes.enumSized (@typ) _ init_size)
-                             (fun 'v5144_ =>
-                              @QuickChick.Enumerators.returnEnum _
-                                (@Coq.Init.Datatypes.Some _ (@Coq.Init.Datatypes.pair _ _ (@App fe xe) v5144_))))))
-                    (@Coq.Init.Datatypes.cons _
-                       (@QuickChick.Enumerators.bindEnum _ _ (@QuickChick.Classes.enumSized (@nat) _ init_size)
-                          (fun 'n =>
-                           @QuickChick.Enumerators.returnEnum _
-                             (@Coq.Init.Datatypes.Some _ (@Coq.Init.Datatypes.pair _ _ (@Const n) (@TNat)))))
-                       (@Coq.Init.Datatypes.nil _)))))
+                 (@QuickChick.Enumerators.bindEnum _ _ (@rec init_size size')
+                    (fun 't1 =>
+                     @QuickChick.Enumerators.bindEnum _ _ (@rec init_size size')
+                       (fun 't2 => @QuickChick.Enumerators.returnEnum _ (@TArrow t1 t2)))) (@Coq.Init.Datatypes.nil _)))
      end in
- fun size : Coq.Init.Datatypes.nat => @EnumSizedSuchThattyping_IOOEnum size size).
+ fun size : Coq.Init.Datatypes.nat => @EnumSizedtyp_Enum size size) 3).
+  
+  
+Sample ((let GenSizedtyp_Gen :=
+   fix rec (init_size : Coq.Init.Datatypes.nat) (size : Coq.Init.Datatypes.nat) :=
+     match size with
+     | @Coq.Init.Datatypes.O =>
+         @QuickChick.Generators.freq_ _ (@QuickChick.Generators.returnGen _ (@TNat))
+           (@Coq.Init.Datatypes.cons _
+              (@Coq.Init.Datatypes.pair _ _ Coq.Init.Nat.one
+                 (@QuickChick.Generators.thunkGen _ (fun '_ => @QuickChick.Generators.returnGen _ (@TNat)))) 
+              (@Coq.Init.Datatypes.nil _))
+     | @Coq.Init.Datatypes.S size' =>
+         @QuickChick.Generators.freq_ _ (@QuickChick.Generators.returnGen _ (@TNat))
+           (@Coq.Init.Datatypes.cons _
+              (@Coq.Init.Datatypes.pair _ _ Coq.Init.Nat.one
+                 (@QuickChick.Generators.thunkGen _ (fun '_ => @QuickChick.Generators.returnGen _ (@TNat))))
+              (@Coq.Init.Datatypes.cons _
+                 (@Coq.Init.Datatypes.pair _ _ size
+                    (@QuickChick.Generators.thunkGen _
+                       (fun '_ =>
+                        @QuickChick.Generators.bindGen _ _ (@rec init_size size')
+                          (fun 't1 =>
+                           @QuickChick.Generators.bindGen _ _ (@rec init_size size')
+                             (fun 't2 => @QuickChick.Generators.returnGen _ (@TArrow t1 t2)))))) (@Coq.Init.Datatypes.nil _)))
+     end in
+ fun size : Coq.Init.Datatypes.nat => @GenSizedtyp_Gen size size) 4).
+  
+Derive Valid Schedules typing 1 consnum 1 derive "Gen".
+Abort.
+#[global] Instance DecOpt_not {A} `{DecOpt A} : DecOpt (~ A). 
+constructor.
+intros n.
+destruct (A ?? n) eqn: E.
+- exact (Some (negb b)).
+- exact None.
+Defined.
+
+Derive Inductive Schedule bind_typ 2 derive "Gen" opt "true".
+
+Instance DecEq_typ : Dec_Eq typ. 
+dec_eq.
+Defined. Check @bindOpt. 
+
+Sample ((fix GenSizedSuchThatbind_typ_IIO size :=
+   let GenSizedSuchThatbind_typ_IIOGen :=
+     fix rec
+       (init_size : Coq.Init.Datatypes.nat) (size : Coq.Init.Datatypes.nat) (v451_ : @list (@prod (@nat) (@typ))) (v452_ : @nat) :=
+       match size with
+       | @Coq.Init.Datatypes.O =>
+           @QuickChick.Generators.backtrack _
+             (@Coq.Init.Datatypes.cons _
+                (@Coq.Init.Datatypes.pair _ _ Coq.Init.Nat.one
+                   (@QuickChick.Generators.thunkGen _
+                      (fun '_ =>
+                       match v451_ with
+                       | @Coq.Init.Datatypes.cons _ (@Coq.Init.Datatypes.pair _ _ v t) env =>
+                           match
+                             @QuickChick.Decidability.decOpt (@Coq.Init.Logic.eq _ v v452_) _
+                               QuickChick.Decidability.checkable_size_limit
+                           with
+                           | @Coq.Init.Datatypes.Some _ (@Coq.Init.Datatypes.true) =>
+                               @QuickChick.Generators.returnGen _ (@Coq.Init.Datatypes.Some _ t)
+                           | _ => @QuickChick.Generators.returnGen _ (@Coq.Init.Datatypes.None _)
+                           end
+                       | _ => @QuickChick.Generators.returnGen _ (@Coq.Init.Datatypes.None _)
+                       end))) (@Coq.Init.Datatypes.nil _))
+       | @Coq.Init.Datatypes.S size' =>
+           @QuickChick.Generators.backtrack _
+             (@Coq.Init.Datatypes.cons _
+                (@Coq.Init.Datatypes.pair _ _ Coq.Init.Nat.one
+                   (@QuickChick.Generators.thunkGen _
+                      (fun '_ =>
+                       match v451_ with
+                       | @Coq.Init.Datatypes.cons _ (@Coq.Init.Datatypes.pair _ _ v t) env =>
+                           match
+                             @QuickChick.Decidability.decOpt (@Coq.Init.Logic.eq _ v v452_) _
+                               QuickChick.Decidability.checkable_size_limit
+                           with
+                           | @Coq.Init.Datatypes.Some _ (@Coq.Init.Datatypes.true) =>
+                               @QuickChick.Generators.returnGen _ (@Coq.Init.Datatypes.Some _ t)
+                           | _ => @QuickChick.Generators.returnGen _ (@Coq.Init.Datatypes.None _)
+                           end
+                       | _ => @QuickChick.Generators.returnGen _ (@Coq.Init.Datatypes.None _)
+                       end)))
+                (@Coq.Init.Datatypes.cons _
+                   (@Coq.Init.Datatypes.pair _ _ size
+                      (@QuickChick.Generators.thunkGen _
+                         (fun '_ =>
+                          match v451_ with
+                          | @Coq.Init.Datatypes.cons _ (@Coq.Init.Datatypes.pair _ _ v' t') env =>
+                              match
+                                @QuickChick.Decidability.negbOpt
+                                  (@QuickChick.Decidability.decOpt (@eq (@nat) v452_ v') _ QuickChick.Decidability.checkable_size_limit)
+                              with
+                              | @Coq.Init.Datatypes.Some _ (@Coq.Init.Datatypes.true) =>
+                                  @QuickChick.Producer.bindOpt _ _ _ _ (@rec init_size size' env v452_)
+                                    (fun 'v453_ => @QuickChick.Generators.returnGen _ (@Coq.Init.Datatypes.Some _ v453_))
+                              | _ => @QuickChick.Generators.returnGen _ (@Coq.Init.Datatypes.None _)
+                              end
+                          | _ => @QuickChick.Generators.returnGen _ (@Coq.Init.Datatypes.None _)
+                          end))) (@Coq.Init.Datatypes.nil _)))
+       end in
+    @GenSizedSuchThatbind_typ_IIOGen size size) 1 [(1,TNat);(2,TArrow TNat TNat)] 2
+
+).
+
+
+Derive Inductive Schedule bind_typ derive "Check" opt "true". Check @pair. Check typ.
+
+Definition check_bind := (let DecOptbind_typ_IIICheck :=
+   fix rec
+     (init_size : Coq.Init.Datatypes.nat) (size : Coq.Init.Datatypes.nat) (v340_ : @list (@prod (@nat) (@typ))) 
+     (v341_ : @nat) (v342_ : @typ) :=
+     match size with
+     | @Coq.Init.Datatypes.O =>
+         @QuickChick.Decidability.checker_backtrack
+           (@Coq.Init.Datatypes.cons _
+              (fun '_ =>
+               match v340_ with
+               | @Coq.Init.Datatypes.cons _ (@Coq.Init.Datatypes.pair _ _ v t) env =>
+                   @QuickChick.Decidability.andBind
+                     (@QuickChick.Decidability.decOpt (@Coq.Init.Logic.eq _ t v342_) _ QuickChick.Decidability.checkable_size_limit)
+                     (@QuickChick.Decidability.andBind
+                        (@QuickChick.Decidability.decOpt (@Coq.Init.Logic.eq _ v v341_) _ QuickChick.Decidability.checkable_size_limit)
+                        (@Coq.Init.Datatypes.Some Coq.Init.Datatypes.bool Coq.Init.Datatypes.true))
+               | _ => @Coq.Init.Datatypes.Some _ Coq.Init.Datatypes.false
+               end) (@Coq.Init.Datatypes.nil _))
+     | @Coq.Init.Datatypes.S size' =>
+         @QuickChick.Decidability.checker_backtrack
+           (@Coq.Init.Datatypes.cons _
+              (fun '_ =>
+               match v340_ with
+               | @Coq.Init.Datatypes.cons _ (@Coq.Init.Datatypes.pair _ _ v t) env =>
+                   @QuickChick.Decidability.andBind
+                     (@QuickChick.Decidability.decOpt (@Coq.Init.Logic.eq _ t v342_) _ QuickChick.Decidability.checkable_size_limit)
+                     (@QuickChick.Decidability.andBind
+                        (@QuickChick.Decidability.decOpt (@Coq.Init.Logic.eq _ v v341_) _ QuickChick.Decidability.checkable_size_limit)
+                        (@Coq.Init.Datatypes.Some Coq.Init.Datatypes.bool Coq.Init.Datatypes.true))
+               | _ => @Coq.Init.Datatypes.Some _ Coq.Init.Datatypes.false
+               end)
+              (@Coq.Init.Datatypes.cons _
+                 (fun '_ =>
+                  match v340_ with
+                  | @Coq.Init.Datatypes.cons _ (@Coq.Init.Datatypes.pair _ _ v' t') env =>
+                      @QuickChick.Decidability.andBind
+                        (@QuickChick.Decidability.negbOpt
+                           (@QuickChick.Decidability.decOpt (@eq (@nat) v341_ v') _ QuickChick.Decidability.checkable_size_limit))
+                        (@QuickChick.Decidability.andBind (@rec init_size size' env v341_ v342_)
+                           (@Coq.Init.Datatypes.Some Coq.Init.Datatypes.bool Coq.Init.Datatypes.true))
+                  | _ => @Coq.Init.Datatypes.Some _ Coq.Init.Datatypes.false
+                  end) (@Coq.Init.Datatypes.nil _)))
+     end in
+ fun size : Coq.Init.Datatypes.nat => @DecOptbind_typ_IIICheck size size).
+
+Eval cbn in check_bind 0 [(1,TNat)] 1 TNat.
+
+Derive Inductive Schedule bind_typ 2 derive "Gen" opt "true".
+
+Definition gen_bind := ((let GenSizedSuchThatbind_typ_IIOGen :=
+   fix rec (init_size : Coq.Init.Datatypes.nat) (size : Coq.Init.Datatypes.nat) (v355_ : @list (@prod (@nat) (@typ))) (v356_ : @nat) :=
+     match size with
+     | @Coq.Init.Datatypes.O =>
+         @QuickChick.Generators.backtrack _
+           (@Coq.Init.Datatypes.cons _
+              (@Coq.Init.Datatypes.pair _ _ Coq.Init.Nat.one
+                 (@QuickChick.Generators.thunkGen _
+                    (fun '_ =>
+                     match v355_ with
+                     | @Coq.Init.Datatypes.cons _ (@Coq.Init.Datatypes.pair _ _ v t) env =>
+                         match
+                           @QuickChick.Decidability.decOpt (@Coq.Init.Logic.eq _ v v356_) _ QuickChick.Decidability.checkable_size_limit
+                         with
+                         | @Coq.Init.Datatypes.Some _ (@Coq.Init.Datatypes.true) =>
+                             @QuickChick.Generators.returnGen _ (@Coq.Init.Datatypes.Some _ t)
+                         | _ => @QuickChick.Generators.returnGen _ (@Coq.Init.Datatypes.None _)
+                         end
+                     | _ => @QuickChick.Generators.returnGen _ (@Coq.Init.Datatypes.None _)
+                     end))) (@Coq.Init.Datatypes.nil _))
+     | @Coq.Init.Datatypes.S size' =>
+         @QuickChick.Generators.backtrack _
+           (@Coq.Init.Datatypes.cons _
+              (@Coq.Init.Datatypes.pair _ _ Coq.Init.Nat.one
+                 (@QuickChick.Generators.thunkGen _
+                    (fun '_ =>
+                     match v355_ with
+                     | @Coq.Init.Datatypes.cons _ (@Coq.Init.Datatypes.pair _ _ v t) env =>
+                         match
+                           @QuickChick.Decidability.decOpt (@Coq.Init.Logic.eq _ v v356_) _ QuickChick.Decidability.checkable_size_limit
+                         with
+                         | @Coq.Init.Datatypes.Some _ (@Coq.Init.Datatypes.true) =>
+                             @QuickChick.Generators.returnGen _ (@Coq.Init.Datatypes.Some _ t)
+                         | _ => @QuickChick.Generators.returnGen _ (@Coq.Init.Datatypes.None _)
+                         end
+                     | _ => @QuickChick.Generators.returnGen _ (@Coq.Init.Datatypes.None _)
+                     end)))
+              (@Coq.Init.Datatypes.cons _
+                 (@Coq.Init.Datatypes.pair _ _ size
+                    (@QuickChick.Generators.thunkGen _
+                       (fun '_ =>
+                        match v355_ with
+                        | @Coq.Init.Datatypes.cons _ (@Coq.Init.Datatypes.pair _ _ v' t') env =>
+                            match
+                              @QuickChick.Decidability.negbOpt
+                                (@QuickChick.Decidability.decOpt (@eq (@nat) v356_ v') _ QuickChick.Decidability.checkable_size_limit)
+                            with
+                            | @Coq.Init.Datatypes.Some _ (@Coq.Init.Datatypes.true) =>
+                                @QuickChick.Producer.bindOpt _ _ _ _ (@rec init_size size' env v356_)
+                                  (fun 'v357_ => @QuickChick.Generators.returnGen _ (@Coq.Init.Datatypes.Some _ v357_))
+                            | _ => @QuickChick.Generators.returnGen _ (@Coq.Init.Datatypes.None _)
+                            end
+                        | _ => @QuickChick.Generators.returnGen _ (@Coq.Init.Datatypes.None _)
+                        end))) (@Coq.Init.Datatypes.nil _)))
+     end in
+ fun size : Coq.Init.Datatypes.nat => @GenSizedSuchThatbind_typ_IIOGen size size))
+.
+Print gen_bind. Search Dec_Eq.
+
+
+
+QuickChickDebug Debug Off.
+
+Derive Inductive Schedule typing 1 2  derive "Gen" opt "true".
+
+Print GenSizedSuchThattyping_IOO.
+
+Search GenSizedSuchThat typing.
+
+Derive Show for term.
+Derive Show for typ.
+
+Sample (GenSizedSuchThattyping_IOO 3 [(1,TNat)]).
+
+Sample ((((fix GenSizedSuchThattyping_IOO (size : Coq.Init.Datatypes.nat) :=
+   match size with
+   | @Coq.Init.Datatypes.O =>
+       fun v_g307_ : @list (@prod (@nat) (@typ)) => @QuickChick.Generators.returnGen _ (@Coq.Init.Datatypes.None _)
+   | @Coq.Init.Datatypes.S size =>
+       let GenSizedSuchThattyping_IOOGen :=
+         fix rec (init_size : Coq.Init.Datatypes.nat) (size : Coq.Init.Datatypes.nat) (v_g307_ : @list (@prod (@nat) (@typ))) :=
+           match size with
+           | @Coq.Init.Datatypes.O =>
+               @QuickChick.Generators.backtrack _
+                 (@Coq.Init.Datatypes.cons _
+                    (@Coq.Init.Datatypes.pair _ _ Coq.Init.Nat.one
+                       (@QuickChick.Generators.thunkGen _
+                          (fun '_ =>
+                           @QuickChick.Producer.bindOpt _ _ _ _ (@GenSizedSuchThatbind_typ_IOO size v_g307_)
+                             (fun '(@Coq.Init.Datatypes.pair _ _ x v309_) =>
+                              @QuickChick.Generators.returnGen _
+                                (@Coq.Init.Datatypes.Some _ (@Coq.Init.Datatypes.pair _ _ (@Var x) v309_))))))
+                    (@Coq.Init.Datatypes.cons _
+                       (@Coq.Init.Datatypes.pair _ _ Coq.Init.Nat.one
+                          (@QuickChick.Generators.thunkGen _
+                             (fun '_ =>
+                              @QuickChick.Generators.bindGen _ _ (@GenSizednat_ size)
+                                (fun 'n =>
+                                 @QuickChick.Generators.returnGen _
+                                   (@Coq.Init.Datatypes.Some _ (@Coq.Init.Datatypes.pair _ _ (@Const n) (@TNat)))))))
+                       (@Coq.Init.Datatypes.nil _)))
+           | @Coq.Init.Datatypes.S size' =>
+               @QuickChick.Generators.backtrack _
+                 (@Coq.Init.Datatypes.cons _
+                    (@Coq.Init.Datatypes.pair _ _ Coq.Init.Nat.one
+                       (@QuickChick.Generators.thunkGen _
+                          (fun '_ =>
+                           @QuickChick.Producer.bindOpt _ _ _ _ (@GenSizedSuchThatbind_typ_IOO size v_g307_)
+                             (fun '(@Coq.Init.Datatypes.pair _ _ x v309_) =>
+                              @QuickChick.Generators.returnGen _
+                                (@Coq.Init.Datatypes.Some _ (@Coq.Init.Datatypes.pair _ _ (@Var x) v309_))))))
+                    (@Coq.Init.Datatypes.cons _
+                       (@Coq.Init.Datatypes.pair _ _ Coq.Init.Nat.one
+                          (@QuickChick.Generators.thunkGen _
+                             (fun '_ =>
+                              @QuickChick.Generators.bindGen _ _ (@GenSizednat_ size)
+                                (fun 'n =>
+                                 @QuickChick.Generators.returnGen _
+                                   (@Coq.Init.Datatypes.Some _ (@Coq.Init.Datatypes.pair _ _ (@Const n) (@TNat)))))))
+                       (@Coq.Init.Datatypes.cons _
+                          (@Coq.Init.Datatypes.pair _ _ size
+                             (@QuickChick.Generators.thunkGen _
+                                (fun '_ =>
+                                 @QuickChick.Generators.bindGen _ _ (@GenSizedtyp_ size)
+                                   (fun 't =>
+                                    @QuickChick.Generators.bindGen _ _ (@GenSizednat_ size)
+                                      (fun 'x =>
+                                       @QuickChick.Producer.bindOpt _ _ _ _
+                                         (@rec init_size size'
+                                            (@Coq.Init.Datatypes.cons (@prod (@nat) (@typ)) (@Coq.Init.Datatypes.pair (@nat) (@typ) x t)
+                                               v_g307_))
+                                         (fun '(@Coq.Init.Datatypes.pair _ _ body tbody) =>
+                                          @QuickChick.Generators.returnGen _
+                                            (@Coq.Init.Datatypes.Some _ (@Coq.Init.Datatypes.pair _ _ (@Abs x t body) (@TArrow t tbody)))))))))
+                          (@Coq.Init.Datatypes.cons _
+                             (@Coq.Init.Datatypes.pair _ _ size
+                                (@QuickChick.Generators.thunkGen _
+                                   (fun '_ =>
+                                    @QuickChick.Generators.bindGen _ _ (@GenSizedtyp_ size)
+                                      (fun 'v309_ =>
+                                       @QuickChick.Producer.bindOpt _ _ _ _ (@rec init_size size' v_g307_)
+                                         (fun '(@Coq.Init.Datatypes.pair _ _ xe tfrom) =>
+                                          @QuickChick.Producer.bindOpt _ _ _ _
+                                            (@GenSizedSuchThattyping_IOI size v_g307_ (@TArrow tfrom v309_))
+                                            (fun 'fe =>
+                                             @QuickChick.Generators.returnGen _
+                                               (@Coq.Init.Datatypes.Some _ (@Coq.Init.Datatypes.pair _ _ (@App fe xe) v309_))))))))
+                             (@Coq.Init.Datatypes.nil _)))))
+           end in
+       @GenSizedSuchThattyping_IOOGen size size
+   end
+ with GenSizedSuchThatbind_typ_IOO (size : Coq.Init.Datatypes.nat) :=
+   match size with
+   | @Coq.Init.Datatypes.O => fun v341_ : @list (@prod (@nat) (@typ)) => @QuickChick.Generators.returnGen _ (@Coq.Init.Datatypes.None _)
+   | @Coq.Init.Datatypes.S size =>
+       let GenSizedSuchThatbind_typ_IOOGen :=
+         fix rec (init_size : Coq.Init.Datatypes.nat) (size : Coq.Init.Datatypes.nat) (v341_ : @list (@prod (@nat) (@typ))) :=
+           match size with
+           | @Coq.Init.Datatypes.O =>
+               @QuickChick.Generators.backtrack _
+                 (@Coq.Init.Datatypes.cons _
+                    (@Coq.Init.Datatypes.pair _ _ Coq.Init.Nat.one
+                       (@QuickChick.Generators.thunkGen _
+                          (fun '_ =>
+                           match v341_ with
+                           | @Coq.Init.Datatypes.cons _ (@Coq.Init.Datatypes.pair _ _ v t) env =>
+                               @QuickChick.Generators.returnGen _ (@Coq.Init.Datatypes.Some _ (@Coq.Init.Datatypes.pair _ _ v t))
+                           | _ => @QuickChick.Generators.returnGen _ (@Coq.Init.Datatypes.None _)
+                           end))) (@Coq.Init.Datatypes.nil _))
+           | @Coq.Init.Datatypes.S size' =>
+               @QuickChick.Generators.backtrack _
+                 (@Coq.Init.Datatypes.cons _
+                    (@Coq.Init.Datatypes.pair _ _ Coq.Init.Nat.one
+                       (@QuickChick.Generators.thunkGen _
+                          (fun '_ =>
+                           match v341_ with
+                           | @Coq.Init.Datatypes.cons _ (@Coq.Init.Datatypes.pair _ _ v t) env =>
+                               @QuickChick.Generators.returnGen _ (@Coq.Init.Datatypes.Some _ (@Coq.Init.Datatypes.pair _ _ v t))
+                           | _ => @QuickChick.Generators.returnGen _ (@Coq.Init.Datatypes.None _)
+                           end)))
+                    (@Coq.Init.Datatypes.cons _
+                       (@Coq.Init.Datatypes.pair _ _ size
+                          (@QuickChick.Generators.thunkGen _
+                             (fun '_ =>
+                              match v341_ with
+                              | @Coq.Init.Datatypes.cons _ (@Coq.Init.Datatypes.pair _ _ v' t') env =>
+                                  match @DecOptTrue_ size with
+                                  | @Coq.Init.Datatypes.Some _ (@Coq.Init.Datatypes.true) =>
+                                      @QuickChick.Producer.bindOpt _ _ _ _ (@rec init_size size' env)
+                                        (fun '(@Coq.Init.Datatypes.pair _ _ v342_ v343_) =>
+                                         match
+                                           @QuickChick.Decidability.negbOpt
+                                             (@QuickChick.Decidability.decOpt (@eq (@nat) v342_ v') _
+                                                QuickChick.Decidability.checkable_size_limit)
+                                         with
+                                         | @Coq.Init.Datatypes.Some _ (@Coq.Init.Datatypes.true) =>
+                                             @QuickChick.Generators.returnGen _
+                                               (@Coq.Init.Datatypes.Some _ (@Coq.Init.Datatypes.pair _ _ v342_ v343_))
+                                         | _ => @QuickChick.Generators.returnGen _ (@Coq.Init.Datatypes.None _)
+                                         end)
+                                  | _ => @QuickChick.Generators.returnGen _ (@Coq.Init.Datatypes.None _)
+                                  end
+                              | _ => @QuickChick.Generators.returnGen _ (@Coq.Init.Datatypes.None _)
+                              end))) (@Coq.Init.Datatypes.nil _)))
+           end in
+       @GenSizedSuchThatbind_typ_IOOGen size size
+   end
+ with DecOptTrue_ (size : Coq.Init.Datatypes.nat) :=
+   match size with
+   | @Coq.Init.Datatypes.O => @Coq.Init.Datatypes.None _
+   | @Coq.Init.Datatypes.S size =>
+       let DecOptTrue_Check :=
+         fix rec (init_size : Coq.Init.Datatypes.nat) (size : Coq.Init.Datatypes.nat) :=
+           match size with
+           | @Coq.Init.Datatypes.O =>
+               @QuickChick.Decidability.checker_backtrack
+                 (@Coq.Init.Datatypes.cons _ (fun '_ => @Coq.Init.Datatypes.Some Coq.Init.Datatypes.bool Coq.Init.Datatypes.true)
+                    (@Coq.Init.Datatypes.nil _))
+           | @Coq.Init.Datatypes.S size' =>
+               @QuickChick.Decidability.checker_backtrack
+                 (@Coq.Init.Datatypes.cons _ (fun '_ => @Coq.Init.Datatypes.Some Coq.Init.Datatypes.bool Coq.Init.Datatypes.true)
+                    (@Coq.Init.Datatypes.nil _))
+           end in
+       @DecOptTrue_Check size size
+   end
+ with GenSizednat_ (size : Coq.Init.Datatypes.nat) :=
+   match size with
+   | @Coq.Init.Datatypes.O => @QuickChick.Generators.returnGen _ (@O)
+   | @Coq.Init.Datatypes.S size =>
+       let GenSizednat_Gen :=
+         fix rec (init_size : Coq.Init.Datatypes.nat) (size : Coq.Init.Datatypes.nat) :=
+           match size with
+           | @Coq.Init.Datatypes.O =>
+               @QuickChick.Generators.freq_ _ (@QuickChick.Generators.returnGen _ (@O))
+                 (@Coq.Init.Datatypes.cons _
+                    (@Coq.Init.Datatypes.pair _ _ Coq.Init.Nat.one
+                       (@QuickChick.Generators.thunkGen _ (fun '_ => @QuickChick.Generators.returnGen _ (@O))))
+                    (@Coq.Init.Datatypes.nil _))
+           | @Coq.Init.Datatypes.S size' =>
+               @QuickChick.Generators.freq_ _ (@QuickChick.Generators.returnGen _ (@O))
+                 (@Coq.Init.Datatypes.cons _
+                    (@Coq.Init.Datatypes.pair _ _ Coq.Init.Nat.one
+                       (@QuickChick.Generators.thunkGen _ (fun '_ => @QuickChick.Generators.returnGen _ (@O))))
+                    (@Coq.Init.Datatypes.cons _
+                       (@Coq.Init.Datatypes.pair _ _ size
+                          (@QuickChick.Generators.thunkGen _
+                             (fun '_ =>
+                              @QuickChick.Generators.bindGen _ _ (@rec init_size size')
+                                (fun 'mu311_ => @QuickChick.Generators.returnGen _ (@S mu311_))))) (@Coq.Init.Datatypes.nil _)))
+           end in
+       @GenSizednat_Gen size size
+   end
+ with GenSizedtyp_ (size : Coq.Init.Datatypes.nat) :=
+   match size with
+   | @Coq.Init.Datatypes.O => @QuickChick.Generators.returnGen _ (@TNat)
+   | @Coq.Init.Datatypes.S size =>
+       let GenSizedtyp_Gen :=
+         fix rec (init_size : Coq.Init.Datatypes.nat) (size : Coq.Init.Datatypes.nat) :=
+           match size with
+           | @Coq.Init.Datatypes.O =>
+               @QuickChick.Generators.freq_ _ (@QuickChick.Generators.returnGen _ (@TNat))
+                 (@Coq.Init.Datatypes.cons _
+                    (@Coq.Init.Datatypes.pair _ _ Coq.Init.Nat.one
+                       (@QuickChick.Generators.thunkGen _ (fun '_ => @QuickChick.Generators.returnGen _ (@TNat))))
+                    (@Coq.Init.Datatypes.nil _))
+           | @Coq.Init.Datatypes.S size' =>
+               @QuickChick.Generators.freq_ _ (@QuickChick.Generators.returnGen _ (@TNat))
+                 (@Coq.Init.Datatypes.cons _
+                    (@Coq.Init.Datatypes.pair _ _ Coq.Init.Nat.one
+                       (@QuickChick.Generators.thunkGen _ (fun '_ => @QuickChick.Generators.returnGen _ (@TNat))))
+                    (@Coq.Init.Datatypes.cons _
+                       (@Coq.Init.Datatypes.pair _ _ size
+                          (@QuickChick.Generators.thunkGen _
+                             (fun '_ =>
+                              @QuickChick.Generators.bindGen _ _ (@rec init_size size')
+                                (fun 't1 =>
+                                 @QuickChick.Generators.bindGen _ _ (@rec init_size size')
+                                   (fun 't2 => @QuickChick.Generators.returnGen _ (@TArrow t1 t2)))))) (@Coq.Init.Datatypes.nil _)))
+           end in
+       @GenSizedtyp_Gen size size
+   end
+ with GenSizedSuchThattyping_IOI (size : Coq.Init.Datatypes.nat) :=
+   match size with
+   | @Coq.Init.Datatypes.O =>
+       fun (v_g477_ : @list (@prod (@nat) (@typ))) (v479_ : @typ) => @QuickChick.Generators.returnGen _ (@Coq.Init.Datatypes.None _)
+   | @Coq.Init.Datatypes.S size =>
+       let GenSizedSuchThattyping_IOIGen :=
+         fix rec
+           (init_size : Coq.Init.Datatypes.nat) (size : Coq.Init.Datatypes.nat) (v_g477_ : @list (@prod (@nat) (@typ))) (v479_ : @typ) :=
+           match size with
+           | @Coq.Init.Datatypes.O =>
+               @QuickChick.Generators.backtrack _
+                 (@Coq.Init.Datatypes.cons _
+                    (@Coq.Init.Datatypes.pair _ _ Coq.Init.Nat.one
+                       (@QuickChick.Generators.thunkGen _
+                          (fun '_ =>
+                           @QuickChick.Producer.bindOpt _ _ _ _ (@GenSizedSuchThatbind_typ_IOI size v_g477_ v479_)
+                             (fun 'x => @QuickChick.Generators.returnGen _ (@Coq.Init.Datatypes.Some _ (@Var x))))))
+                    (@Coq.Init.Datatypes.cons _
+                       (@Coq.Init.Datatypes.pair _ _ Coq.Init.Nat.one
+                          (@QuickChick.Generators.thunkGen _
+                             (fun '_ =>
+                              match v479_ with
+                              | @TNat =>
+                                  @QuickChick.Generators.bindGen _ _ (@GenSizednat_ size)
+                                    (fun 'n => @QuickChick.Generators.returnGen _ (@Coq.Init.Datatypes.Some _ (@Const n)))
+                              | _ => @QuickChick.Generators.returnGen _ (@Coq.Init.Datatypes.None _)
+                              end))) (@Coq.Init.Datatypes.nil _)))
+           | @Coq.Init.Datatypes.S size' =>
+               @QuickChick.Generators.backtrack _
+                 (@Coq.Init.Datatypes.cons _
+                    (@Coq.Init.Datatypes.pair _ _ Coq.Init.Nat.one
+                       (@QuickChick.Generators.thunkGen _
+                          (fun '_ =>
+                           @QuickChick.Producer.bindOpt _ _ _ _ (@GenSizedSuchThatbind_typ_IOI size v_g477_ v479_)
+                             (fun 'x => @QuickChick.Generators.returnGen _ (@Coq.Init.Datatypes.Some _ (@Var x))))))
+                    (@Coq.Init.Datatypes.cons _
+                       (@Coq.Init.Datatypes.pair _ _ Coq.Init.Nat.one
+                          (@QuickChick.Generators.thunkGen _
+                             (fun '_ =>
+                              match v479_ with
+                              | @TNat =>
+                                  @QuickChick.Generators.bindGen _ _ (@GenSizednat_ size)
+                                    (fun 'n => @QuickChick.Generators.returnGen _ (@Coq.Init.Datatypes.Some _ (@Const n)))
+                              | _ => @QuickChick.Generators.returnGen _ (@Coq.Init.Datatypes.None _)
+                              end)))
+                       (@Coq.Init.Datatypes.cons _
+                          (@Coq.Init.Datatypes.pair _ _ size
+                             (@QuickChick.Generators.thunkGen _
+                                (fun '_ =>
+                                 match v479_ with
+                                 | @TArrow t tbody =>
+                                     @QuickChick.Generators.bindGen _ _ (@GenSizednat_ size)
+                                       (fun 'x =>
+                                        @QuickChick.Producer.bindOpt _ _ _ _
+                                          (@rec init_size size'
+                                             (@Coq.Init.Datatypes.cons (@prod (@nat) (@typ))
+                                                (@Coq.Init.Datatypes.pair (@nat) (@typ) x t) v_g477_) tbody)
+                                          (fun 'body => @QuickChick.Generators.returnGen _ (@Coq.Init.Datatypes.Some _ (@Abs x t body))))
+                                 | _ => @QuickChick.Generators.returnGen _ (@Coq.Init.Datatypes.None _)
+                                 end)))
+                          (@Coq.Init.Datatypes.cons _
+                             (@Coq.Init.Datatypes.pair _ _ size
+                                (@QuickChick.Generators.thunkGen _
+                                   (fun '_ =>
+                                    @QuickChick.Generators.bindGen _ _ (@GenSizedtyp_ size)
+                                      (fun 'tfrom =>
+                                       @QuickChick.Producer.bindOpt _ _ _ _ (@rec init_size size' v_g477_ (@TArrow tfrom v479_))
+                                         (fun 'fe =>
+                                          @QuickChick.Producer.bindOpt _ _ _ _ (@rec init_size size' v_g477_ tfrom)
+                                            (fun 'xe => @QuickChick.Generators.returnGen _ (@Coq.Init.Datatypes.Some _ (@App fe xe))))))))
+                             (@Coq.Init.Datatypes.nil _)))))
+           end in
+       @GenSizedSuchThattyping_IOIGen size size
+   end
+ with GenSizedSuchThatbind_typ_IOI (size : Coq.Init.Datatypes.nat) :=
+   match size with
+   | @Coq.Init.Datatypes.O =>
+       fun (v321_ : @list (@prod (@nat) (@typ))) (v323_ : @typ) => @QuickChick.Generators.returnGen _ (@Coq.Init.Datatypes.None _)
+   | @Coq.Init.Datatypes.S size =>
+       let GenSizedSuchThatbind_typ_IOIGen :=
+         fix rec
+           (init_size : Coq.Init.Datatypes.nat) (size : Coq.Init.Datatypes.nat) (v321_ : @list (@prod (@nat) (@typ))) (v323_ : @typ) :=
+           match size with
+           | @Coq.Init.Datatypes.O =>
+               @QuickChick.Generators.backtrack _
+                 (@Coq.Init.Datatypes.cons _
+                    (@Coq.Init.Datatypes.pair _ _ Coq.Init.Nat.one
+                       (@QuickChick.Generators.thunkGen _
+                          (fun '_ =>
+                           match v321_ with
+                           | @Coq.Init.Datatypes.cons _ (@Coq.Init.Datatypes.pair _ _ v t) env =>
+                               match
+                                 @QuickChick.Decidability.decOpt (@Coq.Init.Logic.eq _ t v323_) _
+                                   QuickChick.Decidability.checkable_size_limit
+                               with
+                               | @Coq.Init.Datatypes.Some _ (@Coq.Init.Datatypes.true) =>
+                                   @QuickChick.Generators.returnGen _ (@Coq.Init.Datatypes.Some _ v)
+                               | _ => @QuickChick.Generators.returnGen _ (@Coq.Init.Datatypes.None _)
+                               end
+                           | _ => @QuickChick.Generators.returnGen _ (@Coq.Init.Datatypes.None _)
+                           end))) (@Coq.Init.Datatypes.nil _))
+           | @Coq.Init.Datatypes.S size' =>
+               @QuickChick.Generators.backtrack _
+                 (@Coq.Init.Datatypes.cons _
+                    (@Coq.Init.Datatypes.pair _ _ Coq.Init.Nat.one
+                       (@QuickChick.Generators.thunkGen _
+                          (fun '_ =>
+                           match v321_ with
+                           | @Coq.Init.Datatypes.cons _ (@Coq.Init.Datatypes.pair _ _ v t) env =>
+                               match
+                                 @QuickChick.Decidability.decOpt (@Coq.Init.Logic.eq _ t v323_) _
+                                   QuickChick.Decidability.checkable_size_limit
+                               with
+                               | @Coq.Init.Datatypes.Some _ (@Coq.Init.Datatypes.true) =>
+                                   @QuickChick.Generators.returnGen _ (@Coq.Init.Datatypes.Some _ v)
+                               | _ => @QuickChick.Generators.returnGen _ (@Coq.Init.Datatypes.None _)
+                               end
+                           | _ => @QuickChick.Generators.returnGen _ (@Coq.Init.Datatypes.None _)
+                           end)))
+                    (@Coq.Init.Datatypes.cons _
+                       (@Coq.Init.Datatypes.pair _ _ size
+                          (@QuickChick.Generators.thunkGen _
+                             (fun '_ =>
+                              match v321_ with
+                              | @Coq.Init.Datatypes.cons _ (@Coq.Init.Datatypes.pair _ _ v' t') env =>
+                                  match @DecOptTrue_ size with
+                                  | @Coq.Init.Datatypes.Some _ (@Coq.Init.Datatypes.true) =>
+                                      @QuickChick.Producer.bindOpt _ _ _ _ (@rec init_size size' env v323_)
+                                        (fun 'v322_ =>
+                                         match
+                                           @QuickChick.Decidability.negbOpt
+                                             (@QuickChick.Decidability.decOpt (@eq (@nat) v322_ v') _
+                                                QuickChick.Decidability.checkable_size_limit)
+                                         with
+                                         | @Coq.Init.Datatypes.Some _ (@Coq.Init.Datatypes.true) =>
+                                             @QuickChick.Generators.returnGen _ (@Coq.Init.Datatypes.Some _ v322_)
+                                         | _ => @QuickChick.Generators.returnGen _ (@Coq.Init.Datatypes.None _)
+                                         end)
+                                  | _ => @QuickChick.Generators.returnGen _ (@Coq.Init.Datatypes.None _)
+                                  end
+                              | _ => @QuickChick.Generators.returnGen _ (@Coq.Init.Datatypes.None _)
+                              end))) (@Coq.Init.Datatypes.nil _)))
+           end in
+       @GenSizedSuchThatbind_typ_IOIGen size size
+   end
+ for
+ GenSizedSuchThattyping_IOO)
+)
+        ) 4 [(1,TNat);(2,TArrow TNat TNat); (3, TNat)]).
+
+
+Derive Inductive Schedule nat derive "Enum" opt "false".
+
+Eval compute in ((fix EnumSizednat_ (size : Coq.Init.Datatypes.nat) :=
+   match size with
+   | @Coq.Init.Datatypes.O => @QuickChick.Enumerators.returnEnum _ (@O)
+   | @Coq.Init.Datatypes.S size =>
+       let EnumSizednat_Enum :=
+         fix rec (init_size : Coq.Init.Datatypes.nat) (size : Coq.Init.Datatypes.nat) :=
+           match size with
+           | @Coq.Init.Datatypes.O =>
+               @QuickChick.Producer.oneOf_ _ _ _ (@QuickChick.Enumerators.returnEnum _ (@O))
+                 (@Coq.Init.Datatypes.cons _ (@QuickChick.Enumerators.returnEnum _ (@O)) (@Coq.Init.Datatypes.nil _))
+           | @Coq.Init.Datatypes.S size' =>
+               @QuickChick.Producer.oneOf_ _ _ _ (@QuickChick.Enumerators.returnEnum _ (@O))
+                 (@Coq.Init.Datatypes.cons _ (@QuickChick.Enumerators.returnEnum _ (@O))
+                    (@Coq.Init.Datatypes.cons _
+                       (@QuickChick.Enumerators.bindEnum _ _ (@rec init_size size')
+                          (fun 'mu818_ => @QuickChick.Enumerators.returnEnum _ (@S mu818_))) (@Coq.Init.Datatypes.nil _)))
+           end in
+       @EnumSizednat_Enum size size
+   end) 3).
